libcrux-ml-dsa/proofs/fstar/extraction/Libcrux_ml_dsa.Constants.fst
@@ -8,11 +8,6 @@ let t_Eta_cast_to_repr (x: t_Eta) =
   | Eta_Two  -> discriminant_Eta_Two
   | Eta_Four  -> discriminant_Eta_Four
 
-let t_Gamma2_cast_to_repr (x: t_Gamma2) =
-  match x <: t_Gamma2 with
-  | Gamma2_V95_232_  -> discriminant_Gamma2_V95_232_
-  | Gamma2_V261_888_  -> discriminant_Gamma2_V261_888_
-
 let error_ring_element_size (bits_per_error_coefficient: usize) =
   (bits_per_error_coefficient *! v_COEFFICIENTS_IN_RING_ELEMENT <: usize) /! sz 8
 
@@ -37,36 +32,12 @@ let verification_key_size (rows_in_a: usize) =
 
 [@@ FStar.Tactics.Typeclasses.tcinstance]
 assume
-val impl': Core.Fmt.t_Debug t_Eta
+val impl': Core.Clone.t_Clone t_Eta
 
 let impl = impl'
 
 [@@ FStar.Tactics.Typeclasses.tcinstance]
 assume
-val impl_1': Core.Clone.t_Clone t_Eta
+val impl_1': Core.Marker.t_Copy t_Eta
 
 let impl_1 = impl_1'
-
-[@@ FStar.Tactics.Typeclasses.tcinstance]
-assume
-val impl_2': Core.Marker.t_Copy t_Eta
-
-let impl_2 = impl_2'
-
-[@@ FStar.Tactics.Typeclasses.tcinstance]
-assume
-val impl_3': Core.Fmt.t_Debug t_Gamma2
-
-let impl_3 = impl_3'
-
-[@@ FStar.Tactics.Typeclasses.tcinstance]
-assume
-val impl_4': Core.Clone.t_Clone t_Gamma2
-
-let impl_4 = impl_4'
-
-[@@ FStar.Tactics.Typeclasses.tcinstance]
-assume
-val impl_5': Core.Marker.t_Copy t_Gamma2
-
-let impl_5 = impl_5'
