libcrux-ml-dsa/proofs/fstar/extraction/Libcrux_ml_dsa.Ml_dsa_generic.Instantiations.Avx2.Avx2_feature.fst
@@ -17,66 +17,6 @@ let _ =
   let open Libcrux_ml_dsa.Simd.Traits in
   ()
 
-let generate_key_pair_v44
-      (randomness: t_Array u8 (sz 32))
-      (signing_key verification_key: t_Slice u8)
-     =
-  let tmp0, tmp1:(t_Slice u8 & t_Slice u8) =
-    Libcrux_ml_dsa.Ml_dsa_generic.generate_key_pair_v44 #Libcrux_ml_dsa.Simd.Avx2.Vector_type.t_AVX2SIMDUnit
-      #Libcrux_ml_dsa.Samplex4.Avx2.t_AVX2Sampler
-      #Libcrux_ml_dsa.Hash_functions.Simd256.t_Shake128x4
-      #Libcrux_ml_dsa.Hash_functions.Simd256.t_Shake256
-      #Libcrux_ml_dsa.Hash_functions.Portable.t_Shake256Xof
-      #Libcrux_ml_dsa.Hash_functions.Simd256.t_Shake256x4
-      randomness
-      signing_key
-      verification_key
-  in
-  let signing_key:t_Slice u8 = tmp0 in
-  let verification_key:t_Slice u8 = tmp1 in
-  let hax_temp_output:Prims.unit = () in
-  signing_key, verification_key <: (t_Slice u8 & t_Slice u8)
-
-let generate_key_pair_v65
-      (randomness: t_Array u8 (sz 32))
-      (signing_key verification_key: t_Slice u8)
-     =
-  let tmp0, tmp1:(t_Slice u8 & t_Slice u8) =
-    Libcrux_ml_dsa.Ml_dsa_generic.generate_key_pair_v65 #Libcrux_ml_dsa.Simd.Avx2.Vector_type.t_AVX2SIMDUnit
-      #Libcrux_ml_dsa.Samplex4.Avx2.t_AVX2Sampler
-      #Libcrux_ml_dsa.Hash_functions.Simd256.t_Shake128x4
-      #Libcrux_ml_dsa.Hash_functions.Simd256.t_Shake256
-      #Libcrux_ml_dsa.Hash_functions.Portable.t_Shake256Xof
-      #Libcrux_ml_dsa.Hash_functions.Simd256.t_Shake256x4
-      randomness
-      signing_key
-      verification_key
-  in
-  let signing_key:t_Slice u8 = tmp0 in
-  let verification_key:t_Slice u8 = tmp1 in
-  let hax_temp_output:Prims.unit = () in
-  signing_key, verification_key <: (t_Slice u8 & t_Slice u8)
-
-let generate_key_pair_v87
-      (randomness: t_Array u8 (sz 32))
-      (signing_key verification_key: t_Slice u8)
-     =
-  let tmp0, tmp1:(t_Slice u8 & t_Slice u8) =
-    Libcrux_ml_dsa.Ml_dsa_generic.generate_key_pair_v87 #Libcrux_ml_dsa.Simd.Avx2.Vector_type.t_AVX2SIMDUnit
-      #Libcrux_ml_dsa.Samplex4.Avx2.t_AVX2Sampler
-      #Libcrux_ml_dsa.Hash_functions.Simd256.t_Shake128x4
-      #Libcrux_ml_dsa.Hash_functions.Simd256.t_Shake256
-      #Libcrux_ml_dsa.Hash_functions.Portable.t_Shake256Xof
-      #Libcrux_ml_dsa.Hash_functions.Simd256.t_Shake256x4
-      randomness
-      signing_key
-      verification_key
-  in
-  let signing_key:t_Slice u8 = tmp0 in
-  let verification_key:t_Slice u8 = tmp1 in
-  let hax_temp_output:Prims.unit = () in
-  signing_key, verification_key <: (t_Slice u8 & t_Slice u8)
-
 let sign
       (v_ROWS_IN_A v_COLUMNS_IN_A v_ROWS_X_COLUMNS v_ETA v_ERROR_RING_ELEMENT_SIZE v_GAMMA1_EXPONENT:
           usize)
