libcrux-ml-dsa/proofs/fstar/extraction/Libcrux_ml_dsa.Simd.Avx2.Arithmetic.fst
@@ -3,12 +3,6 @@ module Libcrux_ml_dsa.Simd.Avx2.Arithmetic
 open Core
 open FStar.Mul
 
-let _ =
-  (* This module has implicit dependencies, here we make them explicit. *)
-  (* The implicit dependencies arise from typeclasses instances. *)
-  let open Libcrux_intrinsics.Avx2_extract in
-  ()
-
 let add (lhs rhs: Libcrux_intrinsics.Avx2_extract.t_Vec256) =
   let hax_temp_output, lhs:(Prims.unit & Libcrux_intrinsics.Avx2_extract.t_Vec256) =
     (), Libcrux_intrinsics.Avx2_extract.mm256_add_epi32 lhs rhs
@@ -103,7 +97,7 @@ let shift_left_then_reduce (v_SHIFT_BY: i32) (simd_unit: Libcrux_intrinsics.Avx2
   in
   simd_unit
 
-let to_unsigned_representatives (t: Libcrux_intrinsics.Avx2_extract.t_Vec256) =
+let to_unsigned_representatives_ret (t: Libcrux_intrinsics.Avx2_extract.t_Vec256) =
   let signs:Libcrux_intrinsics.Avx2_extract.t_Vec256 =
     Libcrux_intrinsics.Avx2_extract.mm256_srai_epi32 31l t
   in
@@ -113,118 +107,11 @@ let to_unsigned_representatives (t: Libcrux_intrinsics.Avx2_extract.t_Vec256) =
         <:
         Libcrux_intrinsics.Avx2_extract.t_Vec256)
   in
-  let t:Libcrux_intrinsics.Avx2_extract.t_Vec256 =
-    Libcrux_intrinsics.Avx2_extract.mm256_add_epi32 t conditional_add_field_modulus
-  in
-  t
+  Libcrux_intrinsics.Avx2_extract.mm256_add_epi32 t conditional_add_field_modulus
 
-let decompose
-      (gamma2: Libcrux_ml_dsa.Constants.t_Gamma2)
-      (r r0 r1: Libcrux_intrinsics.Avx2_extract.t_Vec256)
-     =
-  let r:Libcrux_intrinsics.Avx2_extract.t_Vec256 =
-    Core.Clone.f_clone #Libcrux_intrinsics.Avx2_extract.t_Vec256 #FStar.Tactics.Typeclasses.solve r
-  in
-  let r:Libcrux_intrinsics.Avx2_extract.t_Vec256 = to_unsigned_representatives r in
-  let field_modulus_halved:Libcrux_intrinsics.Avx2_extract.t_Vec256 =
-    Libcrux_intrinsics.Avx2_extract.mm256_set1_epi32 ((Libcrux_ml_dsa.Simd.Traits.v_FIELD_MODULUS -!
-          1l
-          <:
-          i32) /!
-        2l
-        <:
-        i32)
-  in
-  let ceil_of_r_by_128_:Libcrux_intrinsics.Avx2_extract.t_Vec256 =
-    Libcrux_intrinsics.Avx2_extract.mm256_add_epi32 r
-      (Libcrux_intrinsics.Avx2_extract.mm256_set1_epi32 127l
-        <:
-        Libcrux_intrinsics.Avx2_extract.t_Vec256)
-  in
-  let ceil_of_r_by_128_:Libcrux_intrinsics.Avx2_extract.t_Vec256 =
-    Libcrux_intrinsics.Avx2_extract.mm256_srai_epi32 7l ceil_of_r_by_128_
-  in
-  let r1:Libcrux_intrinsics.Avx2_extract.t_Vec256 =
-    match gamma2 <: Libcrux_ml_dsa.Constants.t_Gamma2 with
-    | Libcrux_ml_dsa.Constants.Gamma2_V95_232_  ->
-      let result:Libcrux_intrinsics.Avx2_extract.t_Vec256 =
-        Libcrux_intrinsics.Avx2_extract.mm256_mullo_epi32 ceil_of_r_by_128_
-          (Libcrux_intrinsics.Avx2_extract.mm256_set1_epi32 11275l
-            <:
-            Libcrux_intrinsics.Avx2_extract.t_Vec256)
-      in
-      let result:Libcrux_intrinsics.Avx2_extract.t_Vec256 =
-        Libcrux_intrinsics.Avx2_extract.mm256_add_epi32 result
-          (Libcrux_intrinsics.Avx2_extract.mm256_set1_epi32 (1l <<! 23l <: i32)
-            <:
-            Libcrux_intrinsics.Avx2_extract.t_Vec256)
-      in
-      let result:Libcrux_intrinsics.Avx2_extract.t_Vec256 =
-        Libcrux_intrinsics.Avx2_extract.mm256_srai_epi32 24l result
-      in
-      let mask:Libcrux_intrinsics.Avx2_extract.t_Vec256 =
-        Libcrux_intrinsics.Avx2_extract.mm256_sub_epi32 (Libcrux_intrinsics.Avx2_extract.mm256_set1_epi32
-              43l
-            <:
-            Libcrux_intrinsics.Avx2_extract.t_Vec256)
-          result
-      in
-      let mask:Libcrux_intrinsics.Avx2_extract.t_Vec256 =
-        Libcrux_intrinsics.Avx2_extract.mm256_srai_epi32 31l mask
-      in
-      let not_result:Libcrux_intrinsics.Avx2_extract.t_Vec256 =
-        Libcrux_intrinsics.Avx2_extract.mm256_xor_si256 result mask
-      in
-      Libcrux_intrinsics.Avx2_extract.mm256_and_si256 result not_result
-    | Libcrux_ml_dsa.Constants.Gamma2_V261_888_  ->
-      let result:Libcrux_intrinsics.Avx2_extract.t_Vec256 =
-        Libcrux_intrinsics.Avx2_extract.mm256_mullo_epi32 ceil_of_r_by_128_
-          (Libcrux_intrinsics.Avx2_extract.mm256_set1_epi32 1025l
-            <:
-            Libcrux_intrinsics.Avx2_extract.t_Vec256)
-      in
-      let result:Libcrux_intrinsics.Avx2_extract.t_Vec256 =
-        Libcrux_intrinsics.Avx2_extract.mm256_add_epi32 result
-          (Libcrux_intrinsics.Avx2_extract.mm256_set1_epi32 (1l <<! 21l <: i32)
-            <:
-            Libcrux_intrinsics.Avx2_extract.t_Vec256)
-      in
-      let result:Libcrux_intrinsics.Avx2_extract.t_Vec256 =
-        Libcrux_intrinsics.Avx2_extract.mm256_srai_epi32 22l result
-      in
-      Libcrux_intrinsics.Avx2_extract.mm256_and_si256 result
-        (Libcrux_intrinsics.Avx2_extract.mm256_set1_epi32 15l
-          <:
-          Libcrux_intrinsics.Avx2_extract.t_Vec256)
-  in
-  let alpha:i32 =
-    (cast (Libcrux_ml_dsa.Constants.t_Gamma2_cast_to_repr gamma2 <: isize) <: i32) *! 2l
-  in
-  let r0:Libcrux_intrinsics.Avx2_extract.t_Vec256 =
-    Libcrux_intrinsics.Avx2_extract.mm256_mullo_epi32 r1
-      (Libcrux_intrinsics.Avx2_extract.mm256_set1_epi32 alpha
-        <:
-        Libcrux_intrinsics.Avx2_extract.t_Vec256)
-  in
-  let r0:Libcrux_intrinsics.Avx2_extract.t_Vec256 =
-    Libcrux_intrinsics.Avx2_extract.mm256_sub_epi32 r r0
-  in
-  let mask:Libcrux_intrinsics.Avx2_extract.t_Vec256 =
-    Libcrux_intrinsics.Avx2_extract.mm256_sub_epi32 field_modulus_halved r0
-  in
-  let mask:Libcrux_intrinsics.Avx2_extract.t_Vec256 =
-    Libcrux_intrinsics.Avx2_extract.mm256_srai_epi32 31l mask
-  in
-  let field_modulus_and_mask:Libcrux_intrinsics.Avx2_extract.t_Vec256 =
-    Libcrux_intrinsics.Avx2_extract.mm256_and_si256 mask
-      (Libcrux_intrinsics.Avx2_extract.mm256_set1_epi32 Libcrux_ml_dsa.Simd.Traits.v_FIELD_MODULUS
-        <:
-        Libcrux_intrinsics.Avx2_extract.t_Vec256)
-  in
-  let r0:Libcrux_intrinsics.Avx2_extract.t_Vec256 =
-    Libcrux_intrinsics.Avx2_extract.mm256_sub_epi32 r0 field_modulus_and_mask
-  in
-  r0, r1 <: (Libcrux_intrinsics.Avx2_extract.t_Vec256 & Libcrux_intrinsics.Avx2_extract.t_Vec256)
+let to_unsigned_representatives (t: Libcrux_intrinsics.Avx2_extract.t_Vec256) =
+  let t:Libcrux_intrinsics.Avx2_extract.t_Vec256 = to_unsigned_representatives_ret t in
+  t
 
 let power2round (r0 r1: Libcrux_intrinsics.Avx2_extract.t_Vec256) =
   let r0:Libcrux_intrinsics.Avx2_extract.t_Vec256 = to_unsigned_representatives r0 in
@@ -250,80 +137,6 @@ let power2round (r0 r1: Libcrux_intrinsics.Avx2_extract.t_Vec256) =
     Libcrux_intrinsics.Avx2_extract.mm256_sub_epi32 r0 tmp
   in
   r0, r1 <: (Libcrux_intrinsics.Avx2_extract.t_Vec256 & Libcrux_intrinsics.Avx2_extract.t_Vec256)
-
-let use_hint
-      (gamma2: Libcrux_ml_dsa.Constants.t_Gamma2)
-      (r hint: Libcrux_intrinsics.Avx2_extract.t_Vec256)
-     =
-  let r0, r1:(Libcrux_intrinsics.Avx2_extract.t_Vec256 & Libcrux_intrinsics.Avx2_extract.t_Vec256) =
-    Libcrux_ml_dsa.Simd.Avx2.Vector_type.zero (), Libcrux_ml_dsa.Simd.Avx2.Vector_type.zero ()
-    <:
-    (Libcrux_intrinsics.Avx2_extract.t_Vec256 & Libcrux_intrinsics.Avx2_extract.t_Vec256)
-  in
-  let tmp0, tmp1:(Libcrux_intrinsics.Avx2_extract.t_Vec256 &
-    Libcrux_intrinsics.Avx2_extract.t_Vec256) =
-    decompose gamma2 r r0 r1
-  in
-  let r0:Libcrux_intrinsics.Avx2_extract.t_Vec256 = tmp0 in
-  let r1:Libcrux_intrinsics.Avx2_extract.t_Vec256 = tmp1 in
-  let _:Prims.unit = () in
-  let all_zeros:Libcrux_intrinsics.Avx2_extract.t_Vec256 =
-    Libcrux_intrinsics.Avx2_extract.mm256_setzero_si256 ()
-  in
-  let negate_hints:Libcrux_intrinsics.Avx2_extract.t_Vec256 =
-    Libcrux_intrinsics.Avx2_extract.vec256_blendv_epi32 all_zeros hint r0
-  in
-  let negate_hints:Libcrux_intrinsics.Avx2_extract.t_Vec256 =
-    Libcrux_intrinsics.Avx2_extract.mm256_slli_epi32 1l negate_hints
-  in
-  let hints:Libcrux_intrinsics.Avx2_extract.t_Vec256 =
-    Libcrux_intrinsics.Avx2_extract.mm256_sub_epi32 hint negate_hints
-  in
-  let r1_plus_hints:Libcrux_intrinsics.Avx2_extract.t_Vec256 =
-    Libcrux_intrinsics.Avx2_extract.mm256_add_epi32 r1 hints
-  in
-  let (hint, r1_plus_hints), hax_temp_output:((Libcrux_intrinsics.Avx2_extract.t_Vec256 &
-      Libcrux_intrinsics.Avx2_extract.t_Vec256) &
-    Prims.unit) =
-    match gamma2 <: Libcrux_ml_dsa.Constants.t_Gamma2 with
-    | Libcrux_ml_dsa.Constants.Gamma2_V95_232_  ->
-      let max:Libcrux_intrinsics.Avx2_extract.t_Vec256 =
-        Libcrux_intrinsics.Avx2_extract.mm256_set1_epi32 43l
-      in
-      let r1_plus_hints:Libcrux_intrinsics.Avx2_extract.t_Vec256 =
-        Libcrux_intrinsics.Avx2_extract.vec256_blendv_epi32 r1_plus_hints max r1_plus_hints
-      in
-      let greater_than_or_equal_to_max:Libcrux_intrinsics.Avx2_extract.t_Vec256 =
-        Libcrux_intrinsics.Avx2_extract.mm256_cmpgt_epi32 r1_plus_hints max
-      in
-      let hint:Libcrux_intrinsics.Avx2_extract.t_Vec256 =
-        Libcrux_intrinsics.Avx2_extract.vec256_blendv_epi32 r1_plus_hints
-          all_zeros
-          greater_than_or_equal_to_max
-      in
-      (hint, r1_plus_hints
-        <:
-        (Libcrux_intrinsics.Avx2_extract.t_Vec256 & Libcrux_intrinsics.Avx2_extract.t_Vec256)),
-      ()
-      <:
-      ((Libcrux_intrinsics.Avx2_extract.t_Vec256 & Libcrux_intrinsics.Avx2_extract.t_Vec256) &
-        Prims.unit)
-    | Libcrux_ml_dsa.Constants.Gamma2_V261_888_  ->
-      let hint:Libcrux_intrinsics.Avx2_extract.t_Vec256 =
-        Libcrux_intrinsics.Avx2_extract.mm256_and_si256 r1_plus_hints
-          (Libcrux_intrinsics.Avx2_extract.mm256_set1_epi32 15l
-            <:
-            Libcrux_intrinsics.Avx2_extract.t_Vec256)
-      in
-      (hint, r1_plus_hints
-        <:
-        (Libcrux_intrinsics.Avx2_extract.t_Vec256 & Libcrux_intrinsics.Avx2_extract.t_Vec256)),
-      ()
-      <:
-      ((Libcrux_intrinsics.Avx2_extract.t_Vec256 & Libcrux_intrinsics.Avx2_extract.t_Vec256) &
-        Prims.unit)
-  in
-  hint
 
 let montgomery_multiply (lhs rhs: Libcrux_intrinsics.Avx2_extract.t_Vec256) =
   let field_modulus:Libcrux_intrinsics.Avx2_extract.t_Vec256 =
@@ -424,3 +237,192 @@ let montgomery_multiply_by_constant (lhs: Libcrux_intrinsics.Avx2_extract.t_Vec2
     Libcrux_intrinsics.Avx2_extract.mm256_shuffle_epi32 245l res02
   in
   Libcrux_intrinsics.Avx2_extract.mm256_blend_epi32 170l res02_shifted res13
+
+let decompose (gamma2: i32) (r r0 r1: Libcrux_intrinsics.Avx2_extract.t_Vec256) =
+  let r:Libcrux_intrinsics.Avx2_extract.t_Vec256 = to_unsigned_representatives_ret r in
+  let ceil_of_r_by_128_:Libcrux_intrinsics.Avx2_extract.t_Vec256 =
+    Libcrux_intrinsics.Avx2_extract.mm256_add_epi32 r
+      (Libcrux_intrinsics.Avx2_extract.mm256_set1_epi32 127l
+        <:
+        Libcrux_intrinsics.Avx2_extract.t_Vec256)
+  in
+  let ceil_of_r_by_128_:Libcrux_intrinsics.Avx2_extract.t_Vec256 =
+    Libcrux_intrinsics.Avx2_extract.mm256_srai_epi32 7l ceil_of_r_by_128_
+  in
+  let r1:Libcrux_intrinsics.Avx2_extract.t_Vec256 =
+    match gamma2 <: i32 with
+    | 95232l ->
+      let result:Libcrux_intrinsics.Avx2_extract.t_Vec256 =
+        Libcrux_intrinsics.Avx2_extract.mm256_mullo_epi32 ceil_of_r_by_128_
+          (Libcrux_intrinsics.Avx2_extract.mm256_set1_epi32 11275l
+            <:
+            Libcrux_intrinsics.Avx2_extract.t_Vec256)
+      in
+      let result:Libcrux_intrinsics.Avx2_extract.t_Vec256 =
+        Libcrux_intrinsics.Avx2_extract.mm256_add_epi32 result
+          (Libcrux_intrinsics.Avx2_extract.mm256_set1_epi32 (1l <<! 23l <: i32)
+            <:
+            Libcrux_intrinsics.Avx2_extract.t_Vec256)
+      in
+      let result:Libcrux_intrinsics.Avx2_extract.t_Vec256 =
+        Libcrux_intrinsics.Avx2_extract.mm256_srai_epi32 24l result
+      in
+      let mask:Libcrux_intrinsics.Avx2_extract.t_Vec256 =
+        Libcrux_intrinsics.Avx2_extract.mm256_sub_epi32 (Libcrux_intrinsics.Avx2_extract.mm256_set1_epi32
+              43l
+            <:
+            Libcrux_intrinsics.Avx2_extract.t_Vec256)
+          result
+      in
+      let mask:Libcrux_intrinsics.Avx2_extract.t_Vec256 =
+        Libcrux_intrinsics.Avx2_extract.mm256_srai_epi32 31l mask
+      in
+      let not_result:Libcrux_intrinsics.Avx2_extract.t_Vec256 =
+        Libcrux_intrinsics.Avx2_extract.mm256_xor_si256 result mask
+      in
+      let r1:Libcrux_intrinsics.Avx2_extract.t_Vec256 =
+        Libcrux_intrinsics.Avx2_extract.mm256_and_si256 result not_result
+      in
+      r1
+    | 261888l ->
+      let result:Libcrux_intrinsics.Avx2_extract.t_Vec256 =
+        Libcrux_intrinsics.Avx2_extract.mm256_mullo_epi32 ceil_of_r_by_128_
+          (Libcrux_intrinsics.Avx2_extract.mm256_set1_epi32 1025l
+            <:
+            Libcrux_intrinsics.Avx2_extract.t_Vec256)
+      in
+      let result:Libcrux_intrinsics.Avx2_extract.t_Vec256 =
+        Libcrux_intrinsics.Avx2_extract.mm256_add_epi32 result
+          (Libcrux_intrinsics.Avx2_extract.mm256_set1_epi32 (1l <<! 21l <: i32)
+            <:
+            Libcrux_intrinsics.Avx2_extract.t_Vec256)
+      in
+      let result:Libcrux_intrinsics.Avx2_extract.t_Vec256 =
+        Libcrux_intrinsics.Avx2_extract.mm256_srai_epi32 22l result
+      in
+      let r1:Libcrux_intrinsics.Avx2_extract.t_Vec256 =
+        Libcrux_intrinsics.Avx2_extract.mm256_and_si256 result
+          (Libcrux_intrinsics.Avx2_extract.mm256_set1_epi32 15l
+            <:
+            Libcrux_intrinsics.Avx2_extract.t_Vec256)
+      in
+      r1
+    | _ -> r1
+  in
+  let alpha:i32 = gamma2 *! 2l in
+  let r0_tmp:Libcrux_intrinsics.Avx2_extract.t_Vec256 =
+    Libcrux_intrinsics.Avx2_extract.mm256_mullo_epi32 r1
+      (Libcrux_intrinsics.Avx2_extract.mm256_set1_epi32 alpha
+        <:
+        Libcrux_intrinsics.Avx2_extract.t_Vec256)
+  in
+  let r0_tmp:Libcrux_intrinsics.Avx2_extract.t_Vec256 =
+    Libcrux_intrinsics.Avx2_extract.mm256_sub_epi32 r r0_tmp
+  in
+  let field_modulus_halved:Libcrux_intrinsics.Avx2_extract.t_Vec256 =
+    Libcrux_intrinsics.Avx2_extract.mm256_set1_epi32 ((Libcrux_ml_dsa.Simd.Traits.v_FIELD_MODULUS -!
+          1l
+          <:
+          i32) /!
+        2l
+        <:
+        i32)
+  in
+  let mask:Libcrux_intrinsics.Avx2_extract.t_Vec256 =
+    Libcrux_intrinsics.Avx2_extract.mm256_sub_epi32 field_modulus_halved r0_tmp
+  in
+  let mask:Libcrux_intrinsics.Avx2_extract.t_Vec256 =
+    Libcrux_intrinsics.Avx2_extract.mm256_srai_epi32 31l mask
+  in
+  let field_modulus_and_mask:Libcrux_intrinsics.Avx2_extract.t_Vec256 =
+    Libcrux_intrinsics.Avx2_extract.mm256_and_si256 mask
+      (Libcrux_intrinsics.Avx2_extract.mm256_set1_epi32 Libcrux_ml_dsa.Simd.Traits.v_FIELD_MODULUS
+        <:
+        Libcrux_intrinsics.Avx2_extract.t_Vec256)
+  in
+  let r0:Libcrux_intrinsics.Avx2_extract.t_Vec256 =
+    Libcrux_intrinsics.Avx2_extract.mm256_sub_epi32 r0_tmp field_modulus_and_mask
+  in
+  r0, r1 <: (Libcrux_intrinsics.Avx2_extract.t_Vec256 & Libcrux_intrinsics.Avx2_extract.t_Vec256)
+
+let use_hint (gamma2: i32) (r hint: Libcrux_intrinsics.Avx2_extract.t_Vec256) =
+  let r0, r1:(Libcrux_intrinsics.Avx2_extract.t_Vec256 & Libcrux_intrinsics.Avx2_extract.t_Vec256) =
+    Libcrux_ml_dsa.Simd.Avx2.Vector_type.zero (), Libcrux_ml_dsa.Simd.Avx2.Vector_type.zero ()
+    <:
+    (Libcrux_intrinsics.Avx2_extract.t_Vec256 & Libcrux_intrinsics.Avx2_extract.t_Vec256)
+  in
+  let tmp0, tmp1:(Libcrux_intrinsics.Avx2_extract.t_Vec256 &
+    Libcrux_intrinsics.Avx2_extract.t_Vec256) =
+    decompose gamma2 r r0 r1
+  in
+  let r0:Libcrux_intrinsics.Avx2_extract.t_Vec256 = tmp0 in
+  let r1:Libcrux_intrinsics.Avx2_extract.t_Vec256 = tmp1 in
+  let _:Prims.unit = () in
+  let all_zeros:Libcrux_intrinsics.Avx2_extract.t_Vec256 =
+    Libcrux_intrinsics.Avx2_extract.mm256_setzero_si256 ()
+  in
+  let negate_hints:Libcrux_intrinsics.Avx2_extract.t_Vec256 =
+    Libcrux_intrinsics.Avx2_extract.vec256_blendv_epi32 all_zeros hint r0
+  in
+  let negate_hints:Libcrux_intrinsics.Avx2_extract.t_Vec256 =
+    Libcrux_intrinsics.Avx2_extract.mm256_slli_epi32 1l negate_hints
+  in
+  let hints:Libcrux_intrinsics.Avx2_extract.t_Vec256 =
+    Libcrux_intrinsics.Avx2_extract.mm256_sub_epi32 hint negate_hints
+  in
+  let r1_plus_hints:Libcrux_intrinsics.Avx2_extract.t_Vec256 =
+    Libcrux_intrinsics.Avx2_extract.mm256_add_epi32 r1 hints
+  in
+  let (hint, r1_plus_hints), hax_temp_output:((Libcrux_intrinsics.Avx2_extract.t_Vec256 &
+      Libcrux_intrinsics.Avx2_extract.t_Vec256) &
+    Prims.unit) =
+    match gamma2 <: i32 with
+    | 95232l ->
+      let max:Libcrux_intrinsics.Avx2_extract.t_Vec256 =
+        Libcrux_intrinsics.Avx2_extract.mm256_set1_epi32 43l
+      in
+      let r1_plus_hints:Libcrux_intrinsics.Avx2_extract.t_Vec256 =
+        Libcrux_intrinsics.Avx2_extract.vec256_blendv_epi32 r1_plus_hints max r1_plus_hints
+      in
+      let greater_than_or_equal_to_max:Libcrux_intrinsics.Avx2_extract.t_Vec256 =
+        Libcrux_intrinsics.Avx2_extract.mm256_cmpgt_epi32 r1_plus_hints max
+      in
+      let hint:Libcrux_intrinsics.Avx2_extract.t_Vec256 =
+        Libcrux_intrinsics.Avx2_extract.vec256_blendv_epi32 r1_plus_hints
+          all_zeros
+          greater_than_or_equal_to_max
+      in
+      (hint, r1_plus_hints
+        <:
+        (Libcrux_intrinsics.Avx2_extract.t_Vec256 & Libcrux_intrinsics.Avx2_extract.t_Vec256)),
+      ()
+      <:
+      ((Libcrux_intrinsics.Avx2_extract.t_Vec256 & Libcrux_intrinsics.Avx2_extract.t_Vec256) &
+        Prims.unit)
+    | 261888l ->
+      let hint:Libcrux_intrinsics.Avx2_extract.t_Vec256 =
+        Libcrux_intrinsics.Avx2_extract.mm256_and_si256 r1_plus_hints
+          (Libcrux_intrinsics.Avx2_extract.mm256_set1_epi32 15l
+            <:
+            Libcrux_intrinsics.Avx2_extract.t_Vec256)
+      in
+      (hint, r1_plus_hints
+        <:
+        (Libcrux_intrinsics.Avx2_extract.t_Vec256 & Libcrux_intrinsics.Avx2_extract.t_Vec256)),
+      ()
+      <:
+      ((Libcrux_intrinsics.Avx2_extract.t_Vec256 & Libcrux_intrinsics.Avx2_extract.t_Vec256) &
+        Prims.unit)
+    | _ ->
+      (hint, r1_plus_hints
+        <:
+        (Libcrux_intrinsics.Avx2_extract.t_Vec256 & Libcrux_intrinsics.Avx2_extract.t_Vec256)),
+      Rust_primitives.Hax.never_to_any (Core.Panicking.panic "internal error: entered unreachable code"
+
+          <:
+          Rust_primitives.Hax.t_Never)
+      <:
+      ((Libcrux_intrinsics.Avx2_extract.t_Vec256 & Libcrux_intrinsics.Avx2_extract.t_Vec256) &
+        Prims.unit)
+  in
+  hint
