libcrux-ml-dsa/proofs/fstar/extraction/Libcrux_ml_dsa.Simd.Avx2.Arithmetic.fsti
@@ -3,12 +3,6 @@ module Libcrux_ml_dsa.Simd.Avx2.Arithmetic
 open Core
 open FStar.Mul
 
-let _ =
-  (* This module has implicit dependencies, here we make them explicit. *)
-  (* The implicit dependencies arise from typeclasses instances. *)
-  let open Libcrux_intrinsics.Avx2_extract in
-  ()
-
 val add (lhs rhs: Libcrux_intrinsics.Avx2_extract.t_Vec256)
     : Prims.Pure Libcrux_intrinsics.Avx2_extract.t_Vec256 Prims.l_True (fun _ -> Prims.l_True)
 
@@ -26,16 +20,11 @@ val subtract (lhs rhs: Libcrux_intrinsics.Avx2_extract.t_Vec256)
 val shift_left_then_reduce (v_SHIFT_BY: i32) (simd_unit: Libcrux_intrinsics.Avx2_extract.t_Vec256)
     : Prims.Pure Libcrux_intrinsics.Avx2_extract.t_Vec256 Prims.l_True (fun _ -> Prims.l_True)
 
-val to_unsigned_representatives (t: Libcrux_intrinsics.Avx2_extract.t_Vec256)
+val to_unsigned_representatives_ret (t: Libcrux_intrinsics.Avx2_extract.t_Vec256)
     : Prims.Pure Libcrux_intrinsics.Avx2_extract.t_Vec256 Prims.l_True (fun _ -> Prims.l_True)
 
-val decompose
-      (gamma2: Libcrux_ml_dsa.Constants.t_Gamma2)
-      (r r0 r1: Libcrux_intrinsics.Avx2_extract.t_Vec256)
-    : Prims.Pure
-      (Libcrux_intrinsics.Avx2_extract.t_Vec256 & Libcrux_intrinsics.Avx2_extract.t_Vec256)
-      Prims.l_True
-      (fun _ -> Prims.l_True)
+val to_unsigned_representatives (t: Libcrux_intrinsics.Avx2_extract.t_Vec256)
+    : Prims.Pure Libcrux_intrinsics.Avx2_extract.t_Vec256 Prims.l_True (fun _ -> Prims.l_True)
 
 val power2round (r0 r1: Libcrux_intrinsics.Avx2_extract.t_Vec256)
     : Prims.Pure
@@ -43,13 +32,17 @@ val power2round (r0 r1: Libcrux_intrinsics.Avx2_extract.t_Vec256)
       Prims.l_True
       (fun _ -> Prims.l_True)
 
-val use_hint
-      (gamma2: Libcrux_ml_dsa.Constants.t_Gamma2)
-      (r hint: Libcrux_intrinsics.Avx2_extract.t_Vec256)
-    : Prims.Pure Libcrux_intrinsics.Avx2_extract.t_Vec256 Prims.l_True (fun _ -> Prims.l_True)
-
 val montgomery_multiply (lhs rhs: Libcrux_intrinsics.Avx2_extract.t_Vec256)
     : Prims.Pure Libcrux_intrinsics.Avx2_extract.t_Vec256 Prims.l_True (fun _ -> Prims.l_True)
 
 val montgomery_multiply_by_constant (lhs: Libcrux_intrinsics.Avx2_extract.t_Vec256) (constant: i32)
+    : Prims.Pure Libcrux_intrinsics.Avx2_extract.t_Vec256 Prims.l_True (fun _ -> Prims.l_True)
+
+val decompose (gamma2: i32) (r r0 r1: Libcrux_intrinsics.Avx2_extract.t_Vec256)
+    : Prims.Pure
+      (Libcrux_intrinsics.Avx2_extract.t_Vec256 & Libcrux_intrinsics.Avx2_extract.t_Vec256)
+      Prims.l_True
+      (fun _ -> Prims.l_True)
+
+val use_hint (gamma2: i32) (r hint: Libcrux_intrinsics.Avx2_extract.t_Vec256)
     : Prims.Pure Libcrux_intrinsics.Avx2_extract.t_Vec256 Prims.l_True (fun _ -> Prims.l_True)
